src/Language/PlutusIR/Transform/LetNonRec/Static.v
@@ -4,34 +4,131 @@ Require Import Coq.Program.Basics.
 Require Import Coq.Lists.List.
 Import ListNotations.
 
-Require Import PlutusCert.Language.PlutusIR.Semantics.Static.
-Require Import PlutusCert.Language.PlutusIR.Semantics.Static.Implementations.DeBruijn.
-Import DeBruijnTerm.
+Require PlutusCert.Language.PlutusIR.Semantics.Static.
+Require PlutusCert.Language.PlutusIR.Semantics.Static.Implementations.DeBruijn.
+Require PlutusCert.Language.PlutusIR.Semantics.Static.Implementations.Named.
+
 Require Import PlutusCert.Language.PlutusIR.Conversion.
-Import ConvertFunc.
+
+Module DB.
+
+Import PlutusCert.Language.PlutusIR.Semantics.Static.
+Import PlutusCert.Language.PlutusIR.Semantics.Static.Implementations.DeBruijn.
+Import DeBruijnTerm.
+Import ConvertInductive.
 
 Definition P ctx t1 T := 
-  forall t2 t1' t2', 
+  forall t2 t1' t2' vars, 
     CNR_Term t1' t2' -> 
-    to t1' = Coq.Init.Datatypes.Some t1 -> 
-    to t2' = Coq.Init.Datatypes.Some t2 -> 
+    ConvertTerm vars t1' t1 ->
+    ConvertTerm vars t2' t2 ->
     ctx |-+ t2 : T.
+
+Definition Q ctx c := ctx |-ok_c c.
+
+Definition R ctx b1 := 
+  forall b2 b1' b2' vars,
+    Congruence.Cong_Binding CNR_Term b1' b2' ->
+    ConvertBinding vars b1' b1 ->
+    ConvertBinding vars b2' b2 ->
+    ctx |-ok b2.
+
+Axiom skip : forall P, P.
 
 Theorem CNR_Term__preserves_typing : forall ctx t1 T,
     ctx |-+ t1 : T ->
     P ctx t1 T.
 Proof.
-  eapply has_type_rec.
-  - intros. 
-    unfold P. unfold to. intros.
-    destruct t1'; autorewrite with term_to' in H1.
-    + destruct r.
-      * simpl in H1. autorewrite with term_to' in H1.
-        destruct (bindings_to' [] l).
-        -- rewrite app_nil_r in H1.
-           destruct (term_to' (vars_bound_by_bindings l) t1').
-           ++ inversion H1. subst.
-              inversion X. subst.
-              ** autorewrite with term_to' in H2. simpl in H2.
+  apply has_type_rec with (P := P) (P0 := Q) (P1 := R).
+  - intros.  
+    unfold P.
+    intros.
+    inversion H4. subst.
+    inversion X; subst.
+    + apply skip.
+    + inversion X0. subst. apply skip.
+  - intros.
+    unfold P.
+    intros.
+    inversion H5. subst.
+    rename bs0 into bs1'. rename t0 into t1'. rename bs into bs1. rename t into t1.
+    inversion X. subst.
+    inversion X0. subst.
+    rename bs' into bs2'. rename t' into t2'.
+    inversion H6. subst.
+    rename bs' into bs2. rename t0' into t2.
+    eapply T_LetRec.
+    + auto.
+    + reflexivity.
+    + intros.
+      unfold R in H2.
 Abort.
 
+End DB.
+
+
+
+Module Named.
+
+Import PlutusCert.Language.PlutusIR.Semantics.Static.
+Import PlutusCert.Language.PlutusIR.Semantics.Static.Implementations.Named.
+Import NamedTerm.
+
+Definition P_term ctx t1 T := 
+  forall t2, 
+    CNR_Term t1 t2 -> 
+    ctx |-+ t2 : T.
+
+Definition P_constructor ctx c := ctx |-ok_c c.
+
+Definition P_bindings ctx bs1 :=
+    forall bs2,
+      (ctx |-oks bs1 ->
+      Congruence.Cong_Bindings CNR_Term bs1 bs2 ->
+      ctx |-oks bs2) /\
+      (Congruence.Cong_Bindings CNR_Term bs1 bs2 ->
+      map binds bs1 = map binds bs2).
+
+Definition P_binding ctx b1 := 
+  forall b2,
+    Congruence.Cong_Binding CNR_Term b1 b2 ->
+    ctx |-ok b2.
+
+Axiom skip : forall P, P.
+
+Theorem CNR_Term__preserves_typing : forall ctx t1 T,
+    ctx |-+ t1 : T ->
+    P_term ctx t1 T.
+Proof.
+  apply has_type_rec with (P := P_term) (P0 := P_constructor) (P1 := P_bindings) (P2 := P_binding).
+  - intros.  
+    unfold P_term.
+    intros.
+    inversion X; subst.
+    + apply skip.
+    + inversion X0. subst. 
+      apply T_Let.
+      * assumption.
+      * apply H1. assumption. assumption.
+      * unfold P_bindings in H1. edestruct H1 as [_ Heq]. apply Heq in X1. rewrite <- X1. apply H3. assumption. 
+  - intros.
+    unfold P_term.
+    intros.
+    inversion X. subst.
+    inversion X0. subst.
+    eapply T_LetRec.
+    + auto.
+    + reflexivity.
+    + unfold P_bindings in H2.
+      edestruct H2 as [IHH Heq].
+      apply Heq in X1 as Hsu.
+      rewrite <- Hsu.
+      apply IHH. auto. auto.
+    + unfold P_bindings in H2.
+      edestruct H2 as [_ Heq].
+      apply Heq in X1 as Hsu.
+      rewrite <- Hsu.
+      apply H4.
+      assumption.
+  - 
+Abort.
